the functional correctness proof for signatures.

theories/examples/Sig_Prot.v
@@ -65,25 +65,26 @@ Module Type SignatureProt
 
   Import π1 π2 KG Alg Prim.
 
-  Definition Sig_prot_ifce := 
-    [interface #val #[sign] : 'message → 'pubkey × ('signature × 'bool) ].
+  Definition protocol := 30.
+  Definition Sig_prot_ifce :=
+    [interface #val #[protocol] : 'message → 'pubkey × ('signature × 'bool) ].
 
   Definition Sig_prot : package Sig_locs_real Sig_ifce Sig_prot_ifce
     := [package
-      #def  #[sign] (msg : 'message) : 'pubkey × ('signature × 'bool)
+      #def  #[protocol] (msg : 'message) : 'pubkey × ('signature × 'bool)
       {
         #import {sig #[get_pk] : 'unit → 'pubkey } as get_pk ;;
         #import {sig #[sign] : 'message → 'signature  } as sign ;;
         #import {sig #[verify_sig] : ('signature × 'message) → 'bool } as verify_sig ;;
-  
+
         (* Protocol *)
         pk ← get_pk tt ;;
         sig ← sign msg ;;
         bool ← verify_sig (sig, msg) ;;
         ret (pk, ( sig, bool ))
-      } 
+      }
     ].
-  
+
 
   Equations Sig_prot_real : package Sig_locs_real [interface] Sig_prot_ifce :=
     Sig_prot_real := {package Sig_prot ∘ Sig_real_c }.
@@ -129,7 +130,7 @@ Module Type SignatureProt
     Defined.
 
   Lemma ext_unforge_sig_prot:
-  Sig_prot_real ≈₀ Sig_prot_ideal.
+    Sig_prot_real ≈₀ Sig_prot_ideal.
   Proof.
     eapply (eq_rel_perf_ind_ignore (fset [:: sign_loc])).
     - rewrite /Sig_locs_real/Sig_locs_ideal.
@@ -157,6 +158,90 @@ Module Type SignatureProt
            apply Signature_prop.
       ---- by [move: pre; rewrite /inv_conj; repeat case].
   Qed.
-      
+
+  Module Correctness.
+    Definition prot_res := 100.
+
+    Definition Prot_res_ifce :=
+      [interface #val #[prot_res] : 'message → 'unit ].
+
+
+    Equations prot_result (msg : 'message) : code Sig_locs_real Sig_prot_ifce 'bool :=
+      prot_result msg := {code
+        #import {sig #[protocol] : 'message → 'pubkey × ('signature × 'bool) } as protocol ;;
+        '(pk, t) ← protocol msg;;
+        let '(_, result) := t in
+        ret result
+    }.
+
+    (* FIXME This just cannot simplify because it is not clear what the import is! *)
+    Theorem prot_correct seed msg:
+        Run sampler (prot_result msg) seed = Some true.
+    Proof.
+      simpl.
+    Admitted.
+
+
+    Equations prot_result_pkg : package Sig_locs_real Sig_prot_ifce Prot_res_ifce
+      :=
+      prot_result_pkg := [package
+            #def  #[prot_res] (msg : 'message) : 'unit
+            {
+              #import {sig #[protocol] : 'message → 'pubkey × ('signature × 'bool) } as protocol ;;
+              '(_, t) ← protocol msg;;
+              let '(_, result) := t in
+              ret tt
+            }
+        ].
+
+    (* TODO Why do I need this cast here? *)
+    Definition tt_ : chElement 'unit := tt.
+
+    Equations prot_result_pkg' : package Sig_locs_real Sig_prot_ifce Prot_res_ifce
+      :=
+      prot_result_pkg' := [package
+        #def  #[prot_res] (msg : 'message) : 'unit
+        {
+          #import {sig #[protocol] : 'message → 'pubkey × ('signature × 'bool) } as protocol ;;
+          '(_, t) ← protocol msg;;
+          let '(_, result) := t in
+          #assert (result == true) ;;
+          ret tt_
+        }
+        ].
+
+    Equations prot_result_real : package Sig_locs_real [interface] Prot_res_ifce :=
+      prot_result_real := {package prot_result_pkg ∘ Sig_prot ∘ Sig_real_c }.
+    Next Obligation.
+      ssprove_valid.
+      all: by [apply: fsubsetxx].
+    Defined.
+
+    Equations prot_result_real' : package Sig_locs_real [interface] Prot_res_ifce :=
+      prot_result_real' := {package prot_result_pkg' ∘ Sig_prot ∘ Sig_real_c }.
+    Next Obligation.
+      ssprove_valid.
+      all: by [apply: fsubsetxx].
+    Defined.
+
+    Lemma fun_correct:
+      prot_result_real ≈₀ prot_result_real'.
+    Proof.
+      eapply eq_rel_perf_ind_eq.
+      simplify_eq_rel x.
+      all: simplify_linking; ssprove_code_simpl.
+      repeat ssprove_sync_eq.
+      move => _.
+      ssprove_sync_eq => sk.
+      ssprove_sync_eq => pk.
+      rewrite /tt_.
+      have correct_prop: forall p s m, Ver_sig p (Sign s m) m == true.
+      1: { admit.} (* FIXME specify correctness condition *)
+      rewrite (correct_prop pk sk x) /=.
+      apply r_ret => s0 s1 s0_eq_s1 //=.
+    Qed.
+
+  End Correctness.
+
 End SignatureProt.
 
